ToSyntax: add an error context for desugaring

src/parser/FStar.Parser.AST.fst
@@ -27,6 +27,11 @@ open FStar.Ident
 
 module C = FStar.Parser.Const
 
+let lid_of_modul (m:modul) : lid =
+  match m with
+  | Module(lid, _) -> lid
+  | Interface (lid, _, _) -> lid
+
 let check_id id =
     let first_char = String.substring (string_of_id id) 0 1 in
     if String.lowercase first_char = first_char
